Rewrite using nominal2

Lambda.thy
@@ -1,31 +1,153 @@
 theory Lambda
-  imports Main
+  imports Main "Nominal2.Nominal2" "HOL-Eisbach.Eisbach"
 begin
 
-datatype db
-  = Var nat
-  | App db db (infix "°" 200)
-  | Abs db ("λ_" 300)
+atom_decl ident
 
-primrec lift :: "db ⇒ nat ⇒ db" where
-  lift_Var: "lift (Var i) k = (if i < k then Var i else Var (i+1))"
-| lift_App: "lift (m ° n) k = lift m k ° lift n k"
-| lift_Abs: "lift (λm) k = λlift m (k+1)"
+nominal_datatype lam
+  = Var ident
+  | App lam lam (infix "\<degree>" 200)
+  | Abs x::ident m::lam binds x in m ("\<lambda>[_]. _" 300)
 
-primrec subst :: "db ⇒ nat ⇒ db ⇒ db" ("_[_::=_]" [300, 0, 0] 300) where
-  lift_Var: "(Var i)[k::=e] = (if k < i then Var (i-1) else
-                               if k = i then e else Var i)"
-| lift_App: "(m ° n)[k::=e] = m[k::=e] ° n[k::=e]"
-| lift_Abs: "(λ m)[k::=e] = λ(m[k+1::=lift e 0])"
+lemma shows "(\<lambda>[x]. Var x) = \<lambda>[y]. Var y"
+  by auto
 
-inductive beta :: "db ⇒ db ⇒ bool" (infix "→⇩β" 50) where
-  appL: "m →⇩β m' ⟹ m ° n →⇩β m' ° n"
-| appR: "n →⇩β n' ⟹ m ° n →⇩β m ° n'"
-| abs: "m →⇩β m' ⟹ (λm) →⇩β λm'"
-| beta: "(λm) ° n →⇩β m[0::=n]"
+ML \<open>
+fun graph_aux_tac ctxt =
+  SUBGOAL (fn (subgoal, i) =>
+    (case subgoal of
+      Const (@{const_name Trueprop}, _) $ (Const (@{const_name eqvt}, _) $ Free (f, _)) =>
+        full_simp_tac (
+          ctxt addsimps [@{thm eqvt_def}, Proof_Context.get_thm ctxt (f ^ "_def")]) i
+    | _ => no_tac))
+\<close>
 
-code_pred (modes: i ⇒ o ⇒ bool as reduce') beta .
+method_setup eqvt_graph_aux =
+  \<open>Scan.succeed (fn ctxt : Proof.context => SIMPLE_METHOD' (graph_aux_tac ctxt))\<close>
+  "show equivariance of auxilliary graph construction for nominal functions"
 
-definition "reduce t = Predicate.the (reduce' t)"
+method without_alpha_lst methods m =
+  (match termI in H [simproc del: alpha_lst]: _ \<Rightarrow> \<open>m\<close>)
+
+method Abs_lst =
+  (match premises in
+    "atom ?x \<sharp> c" and P [thin]: "[[atom _]]lst. _ = [[atom _]]lst. _" for c :: "'a::fs" \<Rightarrow>
+      \<open>rule Abs_lst1_fcb2' [where c = c, OF P]\<close>
+  \<bar> P [thin]: "[[atom _]]lst. _ = [[atom _]]lst. _" \<Rightarrow> \<open>rule Abs_lst1_fcb2' [where c = "()", OF P]\<close>)
+
+method pat_comp_aux =
+  (match premises in
+    "x = (_ :: lam) \<Longrightarrow> _" for x \<Rightarrow> \<open>rule lam.strong_exhaust [where y = x and c = x]\<close>
+  \<bar> "x = (Var _, _) \<Longrightarrow> _" for x :: "_ :: fs" \<Rightarrow>
+    \<open>rule lam.strong_exhaust [where y = "fst x" and c = x]\<close>
+  \<bar> "x = (_, Var _) \<Longrightarrow> _" for x :: "_ :: fs" \<Rightarrow>
+    \<open>rule lam.strong_exhaust [where y = "snd x" and c = x]\<close>
+  \<bar> "x = (_, _, Var _) \<Longrightarrow> _" for x :: "_ :: fs" \<Rightarrow>
+    \<open>rule lam.strong_exhaust [where y = "snd (snd x)" and c = x]\<close>)
+
+method pat_comp = (pat_comp_aux; force simp: fresh_star_def fresh_Pair_elim)
+
+method freshness uses fresh =
+  (match conclusion in
+    "_ \<sharp> _" \<Rightarrow> \<open>simp add: fresh_Unit fresh_Pair fresh\<close>
+  \<bar> "_ \<sharp>* _" \<Rightarrow> \<open>simp add: fresh_star_def fresh_Unit fresh_Pair fresh\<close>)
+
+method solve_eqvt_at =
+  (simp add: eqvt_at_def; simp add: perm_supp_eq fresh_star_Pair)+
+
+method nf uses fresh = without_alpha_lst \<open>
+  eqvt_graph_aux, rule TrueI, pat_comp, auto, Abs_lst,
+  auto simp: Abs_fresh_iff pure_fresh perm_supp_eq,
+  (freshness fresh: fresh)+,
+  solve_eqvt_at?\<close>
+
+nominal_function subst :: "lam \<Rightarrow> ident \<Rightarrow> lam \<Rightarrow> lam" ("_[_::=_]" [300, 0, 0] 300) where
+  lift_Var: "(Var i)[y::=s] = (if i = y then s else Var i)"
+| lift_App: "(m \<degree> n)[y::=s] = m[y::=s] \<degree> n[y::=s]"
+| lift_Abs: "atom x\<sharp>(y,s) \<Longrightarrow> (\<lambda>[x]. m)[y::=s] = \<lambda>[x]. (m[y::=s])"
+  by (nf)
+
+nominal_termination (eqvt) by lexicographic_order
+
+inductive beta :: "lam \<Rightarrow> lam \<Rightarrow> bool" (infix "\<rightarrow>\<^sub>\<beta>" 50) where
+  appL: "m \<rightarrow>\<^sub>\<beta> m' \<Longrightarrow> m \<degree> n \<rightarrow>\<^sub>\<beta> m' \<degree> n"
+| appR: "n \<rightarrow>\<^sub>\<beta> n' \<Longrightarrow> m \<degree> n \<rightarrow>\<^sub>\<beta> m \<degree> n'"
+| abs: "m \<rightarrow>\<^sub>\<beta> m' \<Longrightarrow> (\<lambda>[x]. m) \<rightarrow>\<^sub>\<beta> \<lambda>[x]. m'"
+| beta: "atom x\<sharp>n \<Longrightarrow> (\<lambda>[x]. m) \<degree> n \<rightarrow>\<^sub>\<beta> m[x::=n]"
+
+equivariance beta
+
+lemma fresh_subst:
+  "atom x\<sharp>n \<Longrightarrow> x = y \<or> atom x\<sharp>m \<Longrightarrow> atom x\<sharp>(m[y::=n])"
+  apply (nominal_induct m avoiding: x y n rule: lam.strong_induct)
+    apply auto
+  done
+
+lemma fresh_subst':
+  "atom x\<sharp>n \<Longrightarrow> atom x\<sharp>m \<Longrightarrow> atom x\<sharp>m[y::=n]"
+  apply (nominal_induct m avoiding: x y n rule: lam.strong_induct)
+    apply auto
+  done
+
+nominal_inductive beta avoids abs:x | beta:x
+     apply (auto simp add: fresh_star_def fresh_subst)
+  done
+
+abbreviation beta_star :: "lam \<Rightarrow> lam \<Rightarrow> bool" (infix "\<rightarrow>\<^sub>\<beta>\<^sup>*" 50) where
+  "x \<rightarrow>\<^sub>\<beta>\<^sup>* y \<equiv> beta\<^sup>*\<^sup>* x y"
+
+inductive par_beta (infix "\<Rightarrow>\<^sub>\<beta>" 50) where
+  app: "\<lbrakk> m \<Rightarrow>\<^sub>\<beta> m'; n \<Rightarrow>\<^sub>\<beta> n' \<rbrakk> \<Longrightarrow> m \<degree> n \<Rightarrow>\<^sub>\<beta> m' \<degree> n'"
+| abs: "m \<Rightarrow>\<^sub>\<beta> m' \<Longrightarrow> (\<lambda>[x]. m) \<Rightarrow>\<^sub>\<beta> \<lambda>[x]. m'"
+| beta: "\<lbrakk> m \<Rightarrow>\<^sub>\<beta> m'; n \<Rightarrow>\<^sub>\<beta> n' \<rbrakk> \<Longrightarrow> (\<lambda>[x]. m) \<degree> n \<Rightarrow>\<^sub>\<beta> m'[x::=n']"
+
+equivariance par_beta
+
+nominal_inductive par_beta .
+
+abbreviation par_beta_star :: "lam \<Rightarrow> lam \<Rightarrow> bool" (infix "\<Rightarrow>\<^sub>\<beta>\<^sup>*" 50) where
+  "x \<Rightarrow>\<^sub>\<beta>\<^sup>* y \<equiv> par_beta\<^sup>*\<^sup>* x y"
+
+lemma par_beta_fresh:
+  assumes "m \<Rightarrow>\<^sub>\<beta> m'" and "atom x\<sharp>m"
+  shows "atom x\<sharp>m'"
+  using assms
+  apply (nominal_induct rule: par_beta.strong_induct)
+     apply (auto simp: fresh_at_base fresh_subst fresh_subst')
+  done
+
+thm par_beta.induct
+
+lemma abs_eq:
+  assumes "(\<lambda>[x]. m) \<Rightarrow>\<^sub>\<beta> n"
+  obtains t where "n = (\<lambda>[x]. t)" "m \<Rightarrow>\<^sub>\<beta> t"
+  using assms
+proof (nominal_induct "(\<lambda>[x]. m)" n avoiding: m rule: par_beta.strong_induct)
+  case (abs m' m'' x')
+  then show ?case
+    apply (auto simp: Abs1_eq_iff par_beta.eqvt fresh_permute_left)
+    by (metis par_beta.eqvt permute_flip_cancel2 par_beta_fresh)
+qed
+
+lemma
+  assumes "m \<degree> n \<Rightarrow>\<^sub>\<beta> s"
+  shows "(s = m' \<degree> n' \<and> m \<Rightarrow>\<^sub>\<beta> m' \<and> n \<Rightarrow>\<^sub>\<beta> n') \<or> (m = (\<lambda>[x]. t) \<and> s = t[x::=n'] \<and> t \<Rightarrow>\<^sub>\<beta> t' \<and> n \<Rightarrow>\<^sub>\<beta> n')"a
+  using assms
+  apply (nominal_induct "m \<degree> n" s rule: par_beta.strong_induct)
+
+theorem confluent:
+  assumes "m \<Rightarrow>\<^sub>\<beta> m\<^sub>1" and "m \<Rightarrow>\<^sub>\<beta> m\<^sub>2"
+  shows "\<exists>u. m\<^sub>1 \<Rightarrow>\<^sub>\<beta> u \<and> m\<^sub>2 \<Rightarrow>\<^sub>\<beta> u"
+  using assms
+proof (nominal_induct m m\<^sub>1 avoiding: m\<^sub>2 rule: par_beta.strong_induct)
+  case (app m m' n n')
+  then show ?case by metis
+next
+  case (abs m m' x)
+  hence ?case by (metis abs_eq par_beta.abs)
+next
+  case (beta m m' n n' x)
+  then show ?case sorry
+qed
 
 end
